CC/Subcapt.lean
@@ -15,11 +15,17 @@ inductive Subcapt : Ctx n m -> CaptureSet n -> CaptureSet n -> Prop where
 | sc_elem :
   x ∈ C ->
   Subcapt Γ {x} C
+| sc_elem_cap :
+  Subcapt Γ {cap} ⟨ xs , rs , true ⟩
 | sc_var :
   BoundVar Γ x (CType.capt C S) ->
   Subcapt Γ {x} C
 | sc_set :
   (∀ x, x ∈ C1 -> Subcapt Γ {x} C2) ->
+  (∀ x, mem_reach x C1 -> Subcapt Γ ⟨ ∅ , {x} , false ⟩ C2) ->
+  (C1.isUniversal -> Subcapt Γ {cap} C2) ->
   Subcapt Γ C1 C2
 | sc_reach :
   Subcapt Γ {x} ⟨∅, {x}, false⟩
+| sc_reach_cap :
+  Subcapt Γ ⟨∅, {x}, false⟩ {cap}
